verif/trie/representation/key.v
@@ -12,7 +12,8 @@ Require Import DB.prog.
 Definition tkey: type := Tstruct _Key_T noattr.
 Definition tkeybox: type := tptr tkey.
 
-Definition key_rep (sh: share) (key: string) (p: val) (p':val) :=
+Definition key_rep (sh: share) (key: string) (p: val) :=
+  EX p': val,
   data_at sh tkey (p', Vint (Int.repr (Zlength key))) p *
   malloc_token Tsh (tarray tschar (Zlength key)) p' *
   cstring_len Tsh key p'.
@@ -20,24 +21,26 @@ Definition key_rep (sh: share) (key: string) (p: val) (p':val) :=
 Definition keybox_rep (sh: share) (key: option string) (p: val) :=
   match key with
   | Some key =>
-    EX k: val, EX k': val, data_at sh tkeybox k p * key_rep Tsh key k k' * malloc_token Tsh tkey k 
+    EX k: val, data_at sh tkeybox k p * key_rep Tsh key k * malloc_token Tsh tkey k 
   | None =>
     data_at sh tkeybox nullval p
   end.
 
-Lemma keyrep_local_facts (sh: share) (key: string) (p p': val):
-  key_rep sh key p p' |-- !! (isptr p /\ isptr p').
+Lemma keyrep_local_facts (sh: share) (key: string) (p: val):
+  key_rep sh key p |-- !! isptr p.
 Proof.
   unfold key_rep.
+  Intros p'.
   entailer!.
 Qed.
 Hint Resolve keyrep_local_facts: saturate_local.
 
 Lemma keyrep_fold (sh: share) (key: string) (p: val) (p': val):
   data_at sh tkey (p', Vint (Int.repr (Zlength key))) p * malloc_token Tsh (tarray tschar (Zlength key)) p' * cstring_len Tsh key p' |--
-  key_rep sh key p p'.
+  key_rep sh key p.
 Proof.
   unfold key_rep.
+  Exists p'.
   cancel.
 Qed.
 
@@ -58,7 +61,7 @@ Ltac fold_keyrep :=
 
 Lemma fold_keyrep_example (sh: share) (key1 key2: string) (p: val) (p': val):
   0 < Zlength key1 + Zlength key2 <= Int.max_unsigned ->
-  data_at sh tkey (p', Vint (Int.repr (Zlength key1 + Zlength key2))) p * data_at Tsh (tarray tschar (Zlength (key1 ++ key2))) (map Vbyte key1 ++ map Vbyte key2) p' * malloc_token Tsh (tarray tschar (Zlength key1 + Zlength key2)) p' |-- key_rep sh (key1 ++ key2) p p'.
+  data_at sh tkey (p', Vint (Int.repr (Zlength key1 + Zlength key2))) p * data_at Tsh (tarray tschar (Zlength (key1 ++ key2))) (map Vbyte key1 ++ map Vbyte key2) p' * malloc_token Tsh (tarray tschar (Zlength key1 + Zlength key2)) p' |-- key_rep sh (key1 ++ key2) p.
 Proof.
   intros.
   rewrite <- map_app.
