verif/trie/specs.v
@@ -10,6 +10,8 @@ Require Import DB.functional.bordernode.
 Require Import DB.representation.bordernode.
 Require Import DB.representation.key.
 Require Import DB.representation.string.
+Require Import DB.representation.btree.
+Require Import DB.representation.trie.
 
 Require Export DB.prog.
 
@@ -32,9 +34,8 @@ Definition surely_malloc_spec: ident * funspec :=
 Definition UTIL_GetNextKeySlice_spec: ident * funspec :=
   DECLARE _UTIL_GetNextKeySlice
   WITH sh: share, str: val, key: string
-  PRE [ _str OF tptr tschar, _len OF tint ]
-  PROP (readable_share sh;
-        0 <= Zlength key <= keyslice_length)
+  PRE [ _str OF tptr tschar, _len OF tuint ]
+  PROP (readable_share sh)
   LOCAL (temp _str str;
          temp _len (Vint (Int.repr (Zlength key))))
   SEP (cstring_len sh key str)
@@ -155,7 +156,7 @@ Definition BN_GetSuffixValue_spec: ident * funspec :=
 
 Definition BN_TestSuffix_spec: ident * funspec :=
   DECLARE _BN_TestSuffix
-  WITH sh_key: share, key: string, k: val, k':val,
+  WITH sh_key: share, key: string, k: val,
        sh_node: share, bordernode: BorderNode.table, p: val
   PRE [ _bn OF tptr tbordernode, _key OF tptr tkey ]                                    
   PROP (readable_share sh_key;
@@ -163,12 +164,12 @@ Definition BN_TestSuffix_spec: ident * funspec :=
         Zlength key > keyslice_length)
   LOCAL (temp _bn p;
          temp _key k)
-  SEP (key_rep sh_key key k k';
+  SEP (key_rep sh_key key k;
        bordernode_rep sh_node bordernode p)
   POST [ tint ]
   PROP ()
   LOCAL (temp ret_temp (if BorderNode.test_suffix (Some (get_suffix key)) bordernode then Vint Int.one else Vint Int.zero))
-  SEP (key_rep sh_key key k k';
+  SEP (key_rep sh_key key k;
        bordernode_rep sh_node bordernode p).
 
 Definition BN_ExportSuffixValue_spec: ident * funspec :=
@@ -227,7 +228,7 @@ Definition BN_HasSuffix_spec: ident * funspec :=
 
 Definition BN_SetValue_spec: ident * funspec :=
   DECLARE _BN_SetValue
-  WITH sh_key: share, key: string, k: val, k':val,
+  WITH sh_key: share, key: string, k: val,
        sh_node: share, bordernode: BorderNode.table, p: val,
        v: val
   PRE [ _bn OF tptr tbordernode, _key OF tptr tkey, _val OF tptr tvoid ]
@@ -237,12 +238,12 @@ Definition BN_SetValue_spec: ident * funspec :=
          temp _key k;
          temp _val v)
   SEP (bordernode_rep sh_node bordernode p;
-         key_rep sh_key key k k')
+         key_rep sh_key key k)
   POST [ tvoid ]
   PROP ()
   LOCAL ()
   SEP (bordernode_rep sh_node (BorderNode.put_value key v bordernode) p;
-       key_rep sh_key key k k').
+       key_rep sh_key key k).
 
 Definition move_key_spec: ident * funspec :=
   DECLARE _move_key
@@ -253,8 +254,125 @@ Definition move_key_spec: ident * funspec :=
          temp _len (Vint (Int.repr (Zlength key))))
   SEP (cstring_len Tsh key s;
        malloc_token Tsh (tarray tschar (Zlength key)) s)
-  POST [ tptr tkey ] EX k:val, EX k':val,
+  POST [ tptr tkey ] EX k:val,
   PROP ()
   LOCAL (temp ret_temp k)
-  SEP (key_rep Tsh key k k';
+  SEP (key_rep Tsh key k;
        malloc_token Tsh tkey k).
+
+Definition new_cursor_spec: ident * funspec :=
+  DECLARE _new_cursor
+  WITH tt: unit
+  PRE [ ]
+  PROP ()
+  LOCAL ()
+  SEP ()
+  POST [ tptr Trie.tcursor ] EX pc: val,
+  PROP ()
+  LOCAL (temp ret_temp pc)
+  SEP (Trie.cursor_rep [] pc).
+
+Definition push_cursor_spec: ident * funspec :=
+  DECLARE _push_cursor
+  WITH cs: (@Trie.table val * @BTree.cursor val * @BorderNode.table (@Trie.link val) * BorderNode.cursor),
+       pnode_cursor: val, bnode_cursor: val,
+       c: Trie.cursor, pc: val
+  PRE [ _node_cursor OF tptr BTree.tcursor, _bnode_cursor OF tuint, _cursor OF tptr Trie.tcursor ]
+  PROP ()
+  LOCAL (temp _node_cursor pnode_cursor; temp _bnode_cursor bnode_cursor; temp _cursor pc)
+  SEP (Trie.cursor_slice_rep cs (pnode_cursor, bnode_cursor); Trie.cursor_rep c pc)
+  POST [ tvoid ]
+  PROP ()
+  LOCAL ()
+  SEP (Trie.cursor_rep (c ++ [cs]) pc).
+
+Definition pop_cursor_spec: ident * funspec :=
+  DECLARE _pop_cursor
+  WITH c: Trie.cursor, pc: val
+  PRE [ _cursor OF tptr Trie.tcursor ]
+  PROP ()
+  LOCAL (temp _cursor pc)
+  SEP (Trie.cursor_rep c pc)
+  POST [ tvoid ]
+  PROP ()
+  LOCAL ()
+  SEP (Trie.cursor_rep (removelast c) pc).
+
+Definition _make_cursor_spec: ident * funspec :=
+  DECLARE __make_cursor
+  WITH c: @Trie.cursor val, pc: val,
+       k: string, pk: val,
+       t: @Trie.table val, pt: val
+  PRE [ _key OF tptr tkey, _index OF tptr Trie.tindex, _cursor OF tptr Trie.tcursor ]
+  PROP (Trie.table_correct t)
+  LOCAL (temp _key pk; temp _index pt; temp _cursor pc)
+  SEP (Trie.table_rep t pt; key_rep Tsh k pk; Trie.cursor_rep c pc)
+  POST [ tvoid ]
+  PROP ()
+  LOCAL ()
+  SEP (Trie.table_rep t pt; key_rep Tsh k pk; Trie.cursor_rep (c ++ (Trie.make_cursor k t)) pc).
+
+Definition Imake_cursor_spec: ident * funspec :=
+  DECLARE _Imake_cursor
+  WITH k: Z,
+       t: @BTree.table val, pt: val
+  PRE [ _key OF tuint, _index OF tptr BTree.tindex ]
+  PROP (0 <= k <= Int.max_unsigned; BTree.table_correct t)
+  LOCAL (temp _key (Vint (Int.repr k)); temp _index pt)
+  SEP (BTree.table_rep t pt)
+  POST [ tptr BTree.tcursor ] EX pc: val,
+  PROP ()
+  LOCAL (temp ret_temp pc)
+  SEP (BTree.table_rep t pt; BTree.cursor_rep (BTree.make_cursor k t) pc).
+
+Definition Ifree_cursor_spec: ident * funspec :=
+  DECLARE _Ifree_cursor
+  WITH c: @BTree.cursor val, pc: val
+  PRE [ _cursor OF tptr BTree.tcursor ]
+  PROP ()
+  LOCAL (temp _cursor pc)
+  SEP (BTree.cursor_rep c pc)
+  POST [ tvoid ]
+  PROP ()
+  LOCAL ()
+  SEP ().
+
+Definition Iget_key_spec: ident * funspec :=
+  DECLARE _Iget_key
+  WITH c: @BTree.cursor val, pc: val,
+       t: @BTree.table val, pt: val,
+       pk: val
+  PRE [ _cursor OF tptr BTree.tcursor, _index OF tptr BTree.tindex, _key OF tptr tuint ]
+  PROP (BTree.abs_rel c t)
+  LOCAL (temp _cursor pc; temp _index pt; temp _key pk)
+  SEP (BTree.table_rep t pt; BTree.cursor_rep c pc; data_at_ Tsh tuint pk)
+  POST [ tint ]
+  PROP ()
+  LOCAL (temp ret_temp (if BTree.get_key c t then (Vint Int.one) else (Vint Int.zero)))
+  SEP (BTree.table_rep t pt; BTree.cursor_rep c pc;
+       match BTree.get_key c t with
+       | Some k => data_at Tsh tuint (Vint (Int.repr k)) pk
+       | None => data_at_ Tsh tuint pk
+       end).
+
+Definition Iget_value_spec: ident * funspec :=
+  DECLARE _Iget_value
+  WITH c: @BTree.cursor val, pc: val,
+       t: @BTree.table val, pt: val,
+       pv: val
+  PRE [ _cursor OF tptr BTree.tcursor, _index OF tptr BTree.tindex, _value OF tptr (tptr tvoid) ]
+  PROP (BTree.abs_rel c t)
+  LOCAL (temp _cursor pc; temp _index pt; temp _value pv)
+  SEP (BTree.table_rep t pt; BTree.cursor_rep c pc; data_at_ Tsh (tptr tvoid) pv)
+  POST [ tint ]
+  PROP ()
+  LOCAL (temp ret_temp (if BTree.get_value c t then (Vint Int.one) else (Vint Int.zero)))
+  SEP (BTree.table_rep t pt; BTree.cursor_rep c pc;
+       match BTree.get_value c t with
+       | Some v => data_at Tsh (tptr tvoid) v pv
+       | None => data_at_ Tsh (tptr tvoid) pv
+       end).
+
+(* Definition new_key. *)
+
+(* Definition BN_CompareSuffix. *)
