verif/trie/verif/verif_util.v
@@ -19,9 +19,9 @@ Proof.
   forward.
   forward.
   forward_while (EX i:Z, EX res: Z, EX str':val,
-    PROP (0 <= i <= Zlength key;
+    PROP (0 <= i <= keyslice_length;
           res = get_keyslice_aux (sublist 0 i key) (Z.to_nat i) 0;
-          str' = (field_address0 (Tarray tschar (Zlength key) noattr) [ArraySubsc i] str))
+          str' = (field_address0 (Tarray tschar (Zlength key) noattr) [ArraySubsc (Z.min i (Zlength key))] str))
     LOCAL (temp _i (Vint (Int.repr i));
            temp _res (Vint (Int.repr res));
            temp _str str';
@@ -32,6 +32,7 @@ Proof.
   Exists str.
   unfold cstring_len.
   Intros.
+  rewrite Z.min_l by rep_omega.
   entailer!.
   rewrite field_address0_offset by (auto with field_compatible).
   rewrite isptr_offset_val_zero; auto.
@@ -39,93 +40,93 @@ Proof.
   - forward.
     unfold cstring_len.
     Intros.
-    assert_PROP (str' = field_address (tarray tschar (Zlength key)) [ArraySubsc i] str). {
+    forward_if (
+     PROP ()
+     LOCAL (temp _res (Vint (Int.repr (get_keyslice_aux (sublist 0 (i + 1) key) (Z.to_nat (i + 1)) 0)));
+     temp _i (Vint (Int.repr i));
+     temp _str (field_address0 (Tarray tschar (Zlength key) noattr)
+                               [ArraySubsc (Z.min (i + 1) (Zlength key))]
+                               str);
+     temp _len (Vint (Int.repr (Zlength key))))
+     SEP (data_at sh (tarray tschar (Zlength key)) (map Vbyte key) str)).
+    + assert (0 <= Z.min i (Zlength key) < Zlength key)
+        by (split; [apply Z.min_glb; list_solve | rewrite Z.min_l; rep_omega]).
+      assert_PROP (str' = field_address (tarray tschar (Zlength key)) [ArraySubsc (Z.min i (Zlength key))] str). {
+        entailer!.
+        unfold field_address0.
+        unfold field_address.
+        do 2 rewrite if_true by auto with field_compatible.
+        reflexivity.
+      }
+      rewrite H5.
+      forward.
+      forward.
+      forward.
+      rewrite ?Z.min_l in * by rep_omega.
       entailer!.
-      unfold field_address0.
-      unfold field_address.
-      do 2 rewrite if_true by auto with field_compatible.
-      reflexivity.
-    }
-    rewrite H4.
-    forward.
-    forward.
-    forward.
-    forward.
-    Exists (i + 1, get_keyslice_aux (sublist 0 (i + 1) key) (Z.to_nat (i + 1)) 0, (field_address0 (Tarray tschar (Zlength key) noattr) [ArraySubsc (i + 1)] str)).
-    unfold cstring_len. entailer!.
-    split.
-    + rewrite Int.shifted_or_is_add.
-      * f_equal.
-        f_equal.
-        change (8) with (Byte.zwordsize).
-        rewrite <- Byte.modulus_power.
-        rewrite sublist_split with (mid := i) by list_solve.
-        rewrite sublist_len_1 by list_solve.
-        replace i with (Zlength (sublist 0 i key)) at 3 by (rewrite Zlength_sublist; list_solve).
-        rewrite get_keyslice_snoc.
-        f_equal.
-        -- rewrite Int.unsigned_repr by (apply get_keyslice_aux_inrange; omega).
+      split.
+      * rewrite Int.shifted_or_is_add; [ | rep_omega | ].
+        -- f_equal.
+           f_equal.
+           change (8) with (Byte.zwordsize).
+           rewrite <- Byte.modulus_power.
+           rewrite sublist_split with (mid := i) by list_solve.
+           rewrite sublist_len_1 by list_solve.
+           replace i with (Zlength (sublist 0 i key)) at 3 by (rewrite Zlength_sublist; list_solve).
+           rewrite get_keyslice_snoc.
+           rewrite Int.unsigned_repr by (apply get_keyslice_aux_inrange; rep_omega).
+           change 255 with (Z.ones 8).
+           rewrite Z.land_ones by omega.
+           change (2 ^ 8) with 256.
+           pose proof (Z.mod_pos_bound (Byte.signed (Znth i key)) 256 ltac:(rep_omega)).
+           rewrite Int.unsigned_repr by rep_omega.
            rewrite Zlength_sublist by list_solve.
            rewrite Z.sub_0_r.
-           reflexivity.
+           f_equal.
+           rewrite <- (Zdiv.Zmod_small) with (n := 256) at 1 by rep_omega.
+           apply Byte.eqmod_mod_eq; [omega | ].
+           replace 256 with Byte.modulus by rep_omega.
+           apply Byte.eqmod_sym.
+           apply Byte.eqm_signed_unsigned.
         -- change 255 with (Z.ones 8).
            rewrite Z.land_ones by omega.
            change (2 ^ 8) with 256.
            pose proof (Z.mod_pos_bound (Byte.signed (Znth i key)) 256 ltac:(rep_omega)).
            rewrite Int.unsigned_repr by rep_omega.
-           rewrite <- (Zdiv.Zmod_small) with (n := 256) at 1 by rep_omega.
-           apply Byte.eqmod_mod_eq.
-           ++ omega.
-           ++ replace 256 with Byte.modulus by rep_omega.
-              apply Byte.eqmod_sym.
-              apply Byte.eqm_signed_unsigned.
-      * rep_omega.
-      * change 255 with (Z.ones 8).
-        rewrite Z.land_ones by omega.
-        change (2 ^ 8) with 256.
-        pose proof (Z.mod_pos_bound (Byte.signed (Znth i key)) 256 ltac:(rep_omega)).
-        rewrite Int.unsigned_repr by rep_omega.
-        change (two_p 8) with 256.
-        rep_omega.
-    + rewrite sem_add_pi_ptr_special by (apply field_address_isptr; auto with field_compatible).
-      unfold field_address0.
-      unfold field_address.
-      rewrite if_true by auto with field_compatible.
-      rewrite if_true by auto with field_compatible.
-      rewrite offset_offset_val.
-      simpl; f_equal; rep_omega.
-  - assert (i = Zlength key) by rep_omega.
-    subst i.
-    clear H0 HRE.
-    forward_while (EX i:Z, EX res: Z,
-      PROP (Zlength key <= i <= 4;
-            res = get_keyslice_aux key (Z.to_nat i) 0)
-      LOCAL (temp _i (Vint (Int.repr i));
-             temp _res (Vint (Int.repr res));
-             temp _str str';
-             temp _len (Vint (Int.repr (Zlength key))))
-      SEP (cstring_len sh key str)).
-    Exists (Zlength key).
-    Exists res.
+           change (two_p 8) with 256.
+           omega.
+      * rewrite sem_add_pi_ptr_special.
+        -- simpl.
+           rewrite field_address0_offset by auto with field_compatible.
+           rewrite field_address_offset by auto with field_compatible.
+           simpl.
+           rewrite offset_offset_val.
+           f_equal.
+           rep_omega.
+        -- apply field_address_isptr.
+           auto with field_compatible.
+    + forward.
+      rewrite ?Z.min_r in * by rep_omega.
+      entailer!.
+      * f_equal.
+        rewrite Int.shl_mul.
+        rewrite ?sublist_same_gen by rep_omega.
+        rewrite get_keyslice_padding by list_solve.
+        change (Int.shl Int.one (Int.repr 8)) with (Int.repr 256).
+        rewrite mul_repr.
+        f_equal.
+    + forward.
+      Exists (i + 1, (get_keyslice_aux (sublist 0 (i + 1) key) (Z.to_nat (i + 1)) 0), (field_address0 (Tarray tschar (Zlength key) noattr) [ArraySubsc (Z.min (i + 1) (Zlength key))] str)).
+      entailer!.
+      fold_cstring_len.
+      cancel.
+  - forward.
     entailer!.
-    rewrite sublist_same by list_solve.
+    unfold get_keyslice.
+    assert (i = keyslice_length) by rep_omega.
+    subst.
+    rewrite <- get_keyslice_aux_gen by rep_omega.
     reflexivity.
-    + entailer!.
-    + forward.
-      forward.
-      Exists (i + 1, get_keyslice_aux key (Z.to_nat (i + 1)) 0).
-      entailer!.
-      rewrite Int.shl_mul.
-      rewrite get_keyslice_padding by list_solve.
-      change (Int.shl Int.one (Int.repr 8)) with (Int.repr 256).
-      rewrite mul_repr.
-      f_equal.
-    + forward.
-      entailer!.
-      unfold get_keyslice.
-      assert (i = keyslice_length) by rep_omega.
-      subst i.
-      reflexivity.
 Qed.
 
 Lemma body_UTIL_StrEqual: semax_body Vprog Gprog f_UTIL_StrEqual UTIL_StrEqual_spec.
